\documentclass[12pt]{amsart}
\usepackage{amsthm, amsmath, amssymb}
\usepackage{geometry, setspace, graphicx, enumerate, fullpage}
\usepackage{listings}
\onehalfspacing                 

\usepackage[usenames, dvipsnames]{color}
\definecolor{graphblue}{RGB}{52, 138, 189}
\definecolor{graphpurple}{RGB}{122, 104, 166}

\theoremstyle{plain}% default 
\newtheorem{thm}{Theorem}[section] 
\newtheorem{lem}[thm]{Lemma} 
\newtheorem{prop}[thm]{Proposition} 
\newtheorem{exer}[thm]{Exercise} 

\newtheorem*{cor}{Corollary} 

\theoremstyle{definition} 
\newtheorem{defn}[thm]{Definition}
\newtheorem{conj}[thm]{Conjecture}
\newtheorem{exmp}[thm]{Example}

\theoremstyle{remark} 
\newtheorem*{rem}{Remark} 
\newtheorem*{note}{Note} 
\newtheorem{case}{Case} 

\DeclareMathOperator*{\argmax}{arg\,max}
\DeclareMathOperator*{\argmin}{arg\,min}

\lstset{
language=Python,
numbers=left,
numberstyle=\scriptsize,
stepnumber=0,
numbersep=5pt,
showspaces=false,
breaklines=true,
basicstyle=\ttfamily\scriptsize,
frame=single,
commentstyle=\scriptsize,
prebreak=\raisebox{0ex}[0ex][0ex]{\ensuremath{\hookleftarrow}},
showstringspaces=false,
showtabs=false,
identifierstyle=\ttfamily,
stringstyle=\color{Gray},
commentstyle=\color{graphpurple},
keywordstyle=\color{graphblue},
commentstyle=\color{RoyalBlue},
keywordstyle=\color{RedViolet},
tabsize=2
}

\title{Elements of Statistical Learning - Chapter Solutions}								% Document Title
\author{Andrew Tulloch}

\begin{document}
\maketitle
\setcounter{section}{2}

\section{Chapter 3}

\begin{exer}
  Show that the $F$ statistic for dropping a single coefficient from a model is equal to the square of the corresponding $z$-score.
\end{exer}

\begin{proof}
  Recall that the $F$ statistic is defined by the following expression \[
    \frac{(RSS_0 - RSS_1) / (p_1 - p_0)}{RSS_1 / (N - p_1 - 1)}.
  \] where $RSS_0, RSS_1$ and $p_0 + 1, p_1 + 1$ refer to the residual sum of squares and the number of free parameters in the smaller and bigger models, respectively.  Recall also that the $F$ statistic has a $F_{p_1 - p_0, N-p_1 - 1}$ distribution under the null hypothesis that the smaller model is correct.

  Next, recall that the $z$-score of a coefficient is \[
    z_j = \frac{\hat \beta_j}{\hat \sigma \sqrt{v_j}}
  \] and under the null hypothesis that $\beta_j$ is zero, $z_j$ is distributed according to a $t$-distribution with $N-p-1$ degrees of freedom. 

  Hence, by dropping a single coefficient from a model, our $F$ statistic has a $F_{1, N-p - 1}$ where $p + 1$ are the number of parameters in the original model.  Similarly, the corresponding $z$-score is distributed according to a $t_{N-p-1}$ distribution, and thus the square of the $z$-score is distributed according to an $F_{1, N-p-1}$ distribution, as required.
\end{proof}
\begin{exer}
    Given data on two variables $X$ and $Y$, consider fitting a cubic polynomial regression model $f(X) = \sum_{j=0}^{3} \beta_j X^j$.  In addition to plotting the fitted curve, you would like a 95\% confidence band about the curve.  Consider the following two approaches:
\begin{enumerate}
    \item At each point $x_0$, form a 95\% confidence interval for the linear function $a^T \beta = \sum_{j=0}^{3}\beta_j x_0^j$.  
    \item Form a 95\% confidence set for $\beta$ as in (3.15), which in tun generates confidence intervals for $f(x_0)$.  
\end{enumerate}
   How do these approaches differ?  Which band is likely to be wider?  Conduct a small simulation experiment to compare the two methods.
\end{exer}

\begin{proof}
    The key distinction is that in the first case, we form the set of points such that we are 95\% confident that $\hat f(x_0)$ is within this set, whereas in the second method, we are 95\% confident that an arbitrary point is within our confidence interval.  This is the distinction between a \emph{pointwise} approach and a \emph{global} confidence estimate. 
    
    In the pointwise approach, we seek to estimate the variance of an individual prediction - that is, to calculate $\text{Var}(\hat f(x_0) | x_0)$.  Here, we have \begin{align*}
        \sigma_0^2 = \text{Var}(\hat f(x_0) | x_0) &= \text{Var}(x_0^T \hat \beta | x_0) \\
                                    &= x_0^T \text{Var}(\hat \beta) x_0 \\
                                    &= \hat \sigma^2 x_0^T (X^T X)^{-1} x_0.
    \end{align*} where $\hat \sigma^2$ is the estimated variance of the innovations $\epsilon_i$.
    
    
    \begin{figure}
	\centering\includegraphics[width=\textwidth]{./RCode/CubicRegression.png}
    \end{figure}

    We can implement this algorithm in R as follows:
\clearpage
\begin{lstlisting}
    library("ggplot2")
    library("reshape2")

    # Raw data
    simulation.xs <- c(1959, 1960, 1961, 1962, 1963, 1964, 1965, 1966, 1967, 1968, 1969)
    simulation.ys <- c(4835, 4970, 5085, 5160, 5310, 5260, 5235, 5255, 5235, 5210, 5175)
    simulation.df <- data.frame(pop = simulation.ys, year = simulation.xs)

    # Rescale years
    simulation.df$year <- simulation.df$year - 1964

    # Generate regression, construct confidence intervals
    fit <- lm(pop ~ year + I(year^2) + I(year^3), data=simulation.df)
    xs <- seq(-5, 5, 0.1)
    fit.confidence <- predict(fit, data.frame(year=xs), interval="confidence", level=0.95)


    # Create data frame containing variables of interest
    df <- as.data.frame(fit.confidence)
    df$year <- xs
    df = melt(df, id.vars="year")

    p <- ggplot()
    p <- p + geom_line(aes(x=year, y=value, colour=variable),
                       df)
    P <- p + geom_point(aes(x=year, y=pop), 
                        simulation.df)
    p <- p + scale_x_continuous('Year') 
    p <- p + scale_y_continuous('Population')
    p <- p + opts(title="Cubic regression with confidence intervals")
    p <- p + scale_color_brewer(name="Legend",
            labels=c("Fit", 
                     "95% Lower Bound", 
                     "95% Upper Bound"), 
            palette="Set1")
\end{lstlisting}

\end{proof}
\begin{exer}
    Prove the Gauss-Markov theorem: the least squares estimate of a parameter $a^T\beta$ has a variance no bigger than that of any other linear unbiased estimate of $a^T\beta$.

    Secondly, show that if $\hat V$ is the variance-covariance matrix of the least squares estimate of $\beta$ and $\tilde V$ is the variance covariance matrix of any other linear unbiased estimate, then $\hat V \leq \tilde V$, where $B \leq A$ if $A - B$ is positive semidefinite.
\end{exer}
\begin{proof}
    Let $\hat \theta = a^T \hat \beta = a^T(X^TX)^{-1}X^T y$ be the least squares estimate of $a^T \beta$.  Let $\tilde \theta = c^T y$ be any other unbiased linear estimator of $a^T \beta$.  Now, let $d^T = c^T - a^T(X^{-1}X)^{-1}X^T$.  Then as $c^T y$ is unbiased, we must have \begin{align*}
        E(c^T y) &= E\left( a^T(X^{T}X)^{-1}X^T + d^T\right) y \\
                &= a^T\beta + d^T X\beta \\
                &= a^T\beta
    \end{align*} as $c^T y$ is unbiased, which implies that $d^T X = 0$.

    Now we calculate the variance of our estimator.  We have \begin{align*}
        \text{Var}(c^T y) &= c^T \text{Var}(y) c \\
                    &= \sigma^2 c^T c \\
                    &= \sigma^2 \left( a^T(X^{T}X)^{-1}X^T + d^T \right) \left( a^T (X^T X)^{-1} X^T + d^T \right)^T \\
                    &= \sigma^2 \left( a^T (X^T X)^{-1}X^T + d^T\right) \left(X (X^{T}X)^{-1}a + d\right) \\
                    &= \sigma^2 \left( a^T (X^TX)^{-1}X^T X(X^T X)^{-1} a + a^T (X^T X)^{-1} \underbrace{X^T d}_{=0} + \underbrace{d^T X}_{=0}(X^T X)^{-1} a + d^T d \right) \\
                    &= \sigma^2 \left(\underbrace{a^T (X^T X)^{-1} a}_{\text{Var}(\hat \theta)} + \underbrace{d^t d}_{\geq 0} \right)
    \end{align*}

    Thus $\text{Var}(\hat \theta) \leq \text{Var}(\tilde \theta)$ for all other unbiased linear estimators $\tilde \theta$.

    The proof of the matrix version is almost identical, except we replace our vector $d$ with a matrix $D$.  It is then possible to show that $\tilde V = \hat V + D^T D$, and as $D^T D$ is a positive semidefinite matrix for any $D$, we have $\hat V \leq \tilde V$. 
\end{proof}

\begin{exer}
    Show how the vector of least square coefficients can be obtained from a single pass of the Gram-Schmidt procedure.  Represent your solution in terms of the QR decomposition of $X$.  
\end{exer}

\begin{proof}
    Recall that by a single pass of the Gram-Schmidt procedure, we can write our matrix $X$ as \[
        X = Z \Gamma,
        \] where $Z$ contains the orthogonal columns $z_j$, and $\Gamma$ is an upper-diagonal matrix with ones on the diagonal, and $\gamma_{ij} = \frac{\langle z_i, x_j \rangle}{\| z_i \|^2}$. This is a reflection of the fact that by definition, \[
            x_j = z_j + \sum_{k=0}^{j-1} \gamma_{kj} z_k.
            \]

            Now, by the $QR$ decomposition, we can write $X = QR$, where $Q$ is an orthogonal matrix and $R$ is an upper triangular matrix.  We have $Q = Z D^{-1}$ and $R = D\Gamma$, where $D$ is a diagonal matrix  with $D_{jj} = \| z_j \|$.  

    Now, by definition of $\hat \beta$, we have \[
        (X^T X) \hat \beta = X^T y.
        \]  Now, using the $QR$ decomposition, we have \begin{align*}
            (R^T Q^T) (QR) \hat \beta &= R^T Q^T y \\
            R \hat \beta &= Q^T y
        \end{align*}
    As $R$ is upper triangular, we can write \begin{align*}
        R_{pp} \hat \beta_p &= \langle q_p, y \rangle \\
        \| z_p \| \hat \beta_p &= \| z_p \|^{-1} \langle z_p, y \rangle \\
        \hat \beta_p &= \frac{\langle z_p, y \rangle}{\| z_p \|^2}
    \end{align*} in accordance with our previous results.  Now, by back substitution, we can obtain the sequence of regression coefficients $\hat \beta_j$.  As an example, to calculate $\hat \beta_{p-1}$, we have \begin{align*}
        R_{p-1, p-1} \hat \beta_{p-1} + R_{p-1,p} \hat \beta_p &= \langle q_{p-1}, y \rangle \\
        \| z_{p-1} \| \hat \beta_{p-1} + \| z_{p-1} \| \gamma_{p-1,p} \hat \beta_p &= \| z_{p-1} \|^{-1} \langle z_{p-1}, y \rangle 
    \end{align*} and then solving for $\hat \beta_{p-1}$. This process can be repeated for all $\beta_j$, thus obtaining the regression coefficients in one pass of the Gram-Schmidt procedure.
\end{proof}

\begin{exer}
    Consider the ridge regression problem (3.41).  Show that this problem is equivalent to the problem \[
        \hat \beta^c = \argmin_{\beta^c} \left( \sum_{i=1}^{N} \left( y_i - \beta^c_0 - \sum_{j=1}^{p}(x_{ij} - \hat x_j) \beta^c_j \right)^2 + \lambda \sum_{j=1}^{p}{\beta_j^c}^2 \right)^2.
        \]
\end{exer}
\begin{proof}
    Consider rewriting our objective function above as  \[
        L(\beta^c) = \sum_{i=1}^{N}\left(y_i - \left(\beta_0^c - \sum_{j=1}^{p} \bar x_j \beta_j^c \right) - \sum_{j=1}^p x_{ij} \beta_j^c \right)^2 + \lambda \sum_{j=1}^p {\beta_j^2}^2
        \]
    Note that making the substitutions \begin{align*}
        \beta_0 &\mapsto \beta_0^c - \sum_{j=1}^p \hat x_j \beta_j \\
        \beta_j &\mapsto \beta^c_j, j = 1, 2, \dots, p
    \end{align*} that $\hat \beta$ is a minimiser of the original ridge regression equation if $\hat \beta^c$ is a minimiser of our modified ridge regression.  

    The modified solution merely has a shifted intercept term, and all other coefficients remain the same.  
\end{proof}


\end{document}
